generational/spec/GC.Gen.CheneyGraphReadiness.fsti
@@ -1826,9 +1826,12 @@ val chunked_cheney_gc_correct_after_preflight_full_policy_and_post_reachable_ima
           major fp alloc_fuel (PromotionDemand.minor_promotion_demand minor + 1)
           fresh in
        CReach.chunked_roots_valid_nonblue base_roots r.capacity_major_out /\
-       chunked_major_chunks_above_zero_addr r.capacity_major_out /\
-       chunked_major_objects_are_pointer_fields r.capacity_major_out /\
-       CReach.chunked_major_field_zero_no_minor
+        CReach.chunked_roots_valid_nonblue
+          (CRem.chunked_minor_collection_roots minor major base_roots)
+          r.capacity_major_out /\
+        chunked_major_chunks_above_zero_addr r.capacity_major_out /\
+        chunked_major_objects_are_pointer_fields r.capacity_major_out /\
+        CReach.chunked_major_field_zero_no_minor
          minor r.capacity_major_out))
 
 val chunked_cheney_gc_correct_after_preflight_policy_and_post_reachable_image_single_chunk_from_dense_roots
